secure_api/box/functor_box/Box.Key.fst
@@ -22,11 +22,6 @@ module SPEC = Spec.SecretBox
 
 assume val is_random: bytes -> Type0
 
-// Have an abstract(?) key type in here with a leak function attached? Then abstract-alias it in the AE module.
-// Then we can use it in other places if we don't idealize.
-// What refinements to have on the leak function?
-
-
 type log_region (im:index_module) =
   r:MR.rid{disjoint r (get_rgn im)}
 
@@ -41,27 +36,21 @@ noeq type key_t2 (im:index_module) =
 #set-options "--z3rlimit 300 --max_ifuel 1 --max_fuel 0"
 abstract noeq type key_module (im:index_module) =
   | KM:
+    //key_type: (im:index_module -> t:Type0{t==key_t2 im}) ->
     get_index: (k:key_t2 im -> i:id im{k.i = i}) ->
-    get_rawGT: (#i:id im -> (k:key_t2 im) -> GTot (b:bytes{b=k.raw})) -> // Returns the raw bytes of the key. Needed for spec of gen/leak/coerce.
-    gen: (i:id im -> ST (k:key_t2 im{k.i = i}) // The spec should indicate that the result is random
+    get_rawGT: ((k:key_t2 im) -> GTot (b:aes_key{b=k.raw})) -> // Returns the raw bytes of the key. Needed for spec of gen/leak/coerce.
+    invariant: (h:mem -> Type0) ->
+    gen: (i:id im -> ST (k:key_t2 im{k.i = i}) // The spec should indicate that the result is random and that gen is idempotent
       (requires (fun h0 ->
-        fresh im (ID i) h0 \/ honest im (ID i)
-      ))
-      (ensures  (fun h0 k h1 ->
-        h0 == h1
-      ))) ->
-    coerce: (i:id im -> b:bytes -> ST (k:key_t2 im{k.i = i /\ b=k.raw}) //TODO: make Total
-      (requires (fun h0 ->
-        dishonest im (ID i) \/ fresh im (ID i) h0 //TODO: require only dishonest
-      ))
-      (ensures  (fun h0 k h1 ->
-        h0 == h1
-      ))) ->
-    leak: (k:key_t2 im{(dishonest im (ID (get_index k))) \/ ~(b2t ae_ind_cca)} -> (b:bytes{b = k.raw})) -> //TODO: remove not ae_ind_cca
+        (fresh im (ID i) h0 \/ honest im (ID i))
+        /\ invariant h0))
+      (ensures  (fun h0 k h1 -> invariant h1))) ->
+    coerce: (i:id im{dishonest im (ID i)} -> raw:aes_key -> (k:key_t2 im{k.i = i /\ raw=k.raw})) ->
+    leak: (k:key_t2 im{dishonest im (ID (get_index k))} -> (raw:aes_key{raw = k.raw})) ->
     key_module im
 
-let create (im:index_module) (get_index:(k:key_t2 im -> i:id im{k.i = i})) get_rawGT gen coerce leak =
-  KM get_index get_rawGT gen coerce leak
+let create (im:index_module) (get_index:(k:key_t2 im -> i:id im{k.i = i})) get_rawGT invariant gen coerce leak =
+  KM get_index get_rawGT invariant gen coerce leak
 
 val get_index: im:index_module -> km:key_module im -> k:key_t2 im -> i:id im{k.i = i}
 let get_index im km k =
@@ -69,27 +58,20 @@ let get_index im km k =
 
 val gen: (im:index_module) -> (km:key_module im) -> (i:id im) -> ST (k:key_t2 im{k.i = i})
   (requires (fun h0 ->
-    fresh im (ID i) h0 \/ honest im (ID i)
-  ))
-  (ensures  (fun h0 k h1 ->
-    h0 == h1
-    //let modified_regions_fresh_key = (Set.union (Set.singleton am.message_log_region) (Set.singleton am.key_log_region)) in
-    //(MM.fresh am.key_log i h0 ==> modifies modified_regions_fresh_key h0 h1)
-    ///\ (MM.defined am.key_log i h0 ==> h0 == h1)
-  ))
+    (fresh im (ID i) h0 \/ honest im (ID i))
+    /\ km.invariant h0))
+  (ensures  (fun h0 k h1 -> km.invariant h1))
 let gen im km i =
   km.gen i
 
-val coerce: (im:index_module) -> (km:key_module im) -> (i:id im) -> (b:bytes) -> ST (k:key_t2 im{k.i = i /\ b = k.raw})
-  (requires (fun h0 ->
-    dishonest im (ID i) \/ fresh im (ID i) h0
-  ))
-  (ensures (fun h0 k h1 ->
-    h0 == h1
-  ))
+val coerce: (im:index_module) -> (km:key_module im) -> (i:id im{dishonest im (ID i)}) -> (b:bytes) -> (k:key_t2 im{k.i = i /\ b = k.raw})
 let coerce im km i b =
   km.coerce i b
 
-val leak: im:index_module -> (km:key_module im) -> (k:key_t2 im{(dishonest im (ID k.i)) \/ ~(b2t ae_ind_cca)}) -> (b:bytes{b=k.raw})
+val leak: im:index_module -> (km:key_module im) -> (k:key_t2 im{dishonest im (ID k.i)}) -> (b:bytes{b=k.raw})
 let leak im km k =
   km.leak k
+
+val km_invariant: im:index_module -> km:key_module im -> h0:mem -> Type0
+let km_invariant im km h0 =
+  km.invariant h0
